iris/DinodeSlot.v
@@ -381,11 +381,11 @@ Local Lemma iu_align_arith (kk qq off dv : Z) :
 Proof.
   intros H1 H2 H3 H4 H5 H6 Hd Hoff. split_and!; [| lia | lia].
   assert (Hz : 2147582608 + 1112 * kk + (88 + (64 * qq + off))
-               = (536895628 + 278 * kk + 16 * qq) * 4 + off) by lia.
+               = (536895674 + 278 * kk + 16 * qq) * 4 + off) by lia.
   rewrite Hz. destruct Hd as [-> | ->].
   - rewrite Z.add_mod; [| lia]. rewrite Hoff.
-    replace ((536895628 + 278 * kk + 16 * qq) * 4) with
-      ((536895628 + 278 * kk + 16 * qq) * 2 * 2) by lia.
+    replace ((536895674 + 278 * kk + 16 * qq) * 4) with
+      ((536895674 + 278 * kk + 16 * qq) * 2 * 2) by lia.
     rewrite Z_mod_mult. reflexivity.
   - rewrite Z.add_mod; [| lia]. rewrite Hoff Z_mod_mult. reflexivity.
 Qed.
@@ -406,7 +406,7 @@ Proof.
               ltac:(lia) ltac:(unfold NBUF in Hk; lia) ltac:(lia) ltac:(lia)
               ltac:(lia) ltac:(lia) Hdv Hm)
     as (Hmod & Hlo & Hhi).
-  replace (0x800181c0 + 24 + 1112 * Z.of_nat k + Z.of_nat (88 + (64 * q + off)))
+  replace (0x80018278 + 24 + 1112 * Z.of_nat k + Z.of_nat (88 + (64 * q + off)))
     with (2147582608 + 1112 * Z.of_nat k
           + (88 + (64 * Z.of_nat q + Z.of_nat off))) by lia.
   apply iu_align_z; [exact Hlo | exact Hhi | destruct Hdv as [-> | ->]; lia
