iris/ProofFileinit.v
@@ -87,8 +87,8 @@ Section ProofFileinit.
                                                                                 ltac:(vm_compute; discriminate) Hftable
                   with "Hkdata") as "#Hstr".
     iApply (ILW.wp_initlock_wrapper_sconf KT1 m K KernelSyms.fileinit
-              (mword_of_int 3) (mword_of_int 30) (mword_of_int 1256) (mword_of_int 1032)
-              (mword_of_int 2083468) lk name "ftable"%string vlock vname vcpu b p HK
+              (mword_of_int 3) (mword_of_int 30) (mword_of_int 1060) (mword_of_int 996)
+              (mword_of_int 2083436) lk name "ftable"%string vlock vname vcpu b p HK
               ltac:(vm_compute; reflexivity)
               ltac:(apply bv_eq; vm_compute; reflexivity)
               ltac:(apply bv_eq; vm_compute; reflexivity)
